WIP

src/example/ClientSpinlock2.v
@@ -203,7 +203,7 @@ Section SIM.
                    (▿ γκl γκw) ∗ (△ γκw (1/2)) ∗ (Duty(tid) [(κw, 0, (∃ (γκu : τ{nat}), ▿ γκw γκu))]) ∗ ◇[κw](ℓl, 1)
                )%S : sProp n).
     iSpecialize ("SPEC" $! _ P0 R0 Q0 1).
-    iApply ("SPEC" with "[PC2 LIVE_l DUTY] [TID PCS]").
+    iApply ("SPEC" with "[PC2 LIVE_l DUTY] [TID]").
 
     (* PRE. *)
     { Local Opaque env_live_chain.
@@ -223,6 +223,7 @@ Section SIM.
         iEval (unfold clientSpinlock2_inv; simpl; red_tl_all; simpl) in "CL".
         iDestruct "CL" as "[CL1 | [CL2 | [CL3 | CL4]]]".
         - iExFalso. iDestruct "CL1" as "(LXw & _)". iPoseProof (AuthExcls.b_w_eq with "LX LXw") as "%F". inv F.
+
         - iDestruct "CL2" as "(LXw & PTD & %κw & CL2)". iEval (red_tl) in "CL2". iDestruct "CL2" as "[%γκw CL2]".
           iEval (red_tl_all; simpl) in "CL2". iDestruct "CL2" as "(#PROM_w & LIVE_w & #DEAD_l & DUTY2 & PC_spin & LO_w)".
           iDestruct "LO_w" as "[% LO]". iEval (red_tl; simpl) in "LO". iPoseProof "LO" as "[#LO %LAY]".
@@ -237,40 +238,62 @@ Section SIM.
             { iEval (unfold spinlockInv; red_tl_all; simpl) in "INV_SL_CLOSE". iFrame. }
             iRight. iFrame.
           }
-          iExists κw, x, (((⤉ syn_inv n N_Spinlock (spinlockInv n X γX γe)) ∗ ((⤉ spinlockInv n X γX γe =| S n |={ ⊤ ∖ ↑N_Spinlock, ⊤ }=∗ emp) ∗ ⤉ spinlockInv n X γX γe)) ∗ (⤉ -[κw](0)-◇ (∃ (γκu : τ{nat}), ▿ γκw γκu)) ∗ (⤉ ▿ γκl γκw))%S.
+          iExists κw, x, (((⤉ syn_inv n N_Spinlock (spinlockInv n X γX γe)) ∗ ((⤉ spinlockInv n X γX γe =| S n |={ ⊤ ∖ ↑N_Spinlock, ⊤ }=∗ emp) ∗ ⤉ spinlockInv n X γX γe)) ∗ (⤉ (∃ (γκu : τ{nat}), ▿ γκw γκu)))%S.
           iSplitR. auto. iSplitR. auto. iSplitR.
           { iModIntro. iIntros "B". iModIntro. iEval (red_tl; simpl) in "B". iDestruct "B" as "(A & C)".
             iSplitL "A".
             { iEval (red_tl). iFrame. }
-            iModIntro. iEval (red_tl). iIntros "A".
-
-            TODO
-
-          
-           S n ⟧ ∗
-
-                         )%S.
-            iFrame.
-            iRight. iFrame.
-          
-
-
-          iDestruct "CL2" as "(LXw & PTD & %κw & CL2)". iEval (red_tl) in "CL2". iDestruct "CL2" as "[%γκw CL2]".
-          iEval (red_tl_all; simpl) in "CL2". iDestruct "CL2" as "(#PROM_w & LIVE_w & #DEAD_l & DUTY2 & PC_spin & LO_w)".
-          iMod (tpromise_progress with "[FC]") as "[PC_w | #FULF_w]".
-          { iFrame. iApply "PROM_w". }
-          { iMod (link_amplify with "[PC_w]") as "PC_s".
-            { iFrame. iApply "LINK_w". }
-            iMod ("INV_CL_CLOSE" with "[LXw PTD LIVE_w PC_spin DUTY2 LO_w]") as "_".
-            { iEval (unfold clientSpinlock2_inv; simpl; red_tl_all; simpl). iRight. iLeft. iFrame.
-              iExists _. iEval (red_tl_all). iExists _. iEval (red_tl_all; simpl). iFrame. iSplit. iApply "PROM_w". iSplit; auto.
+            iModIntro. iEval (red_tl; simpl). iIntros "A". iModIntro. iFrame.
+          }
+          Local Transparent env_live_chain0.
+          iSplitR.
+          { (* ELC at 0. *)
+            iModIntro. iEval (simpl; red_tl; simpl). iIntros "FC A".
+            iMod (tpromise_progress with "[FC]") as "[PC_w | #FULF_w]".
+            { iSplitR. iApply "PROM_w". iFrame. }
+            { iModIntro. iLeft. iFrame. }
+            { iEval (simpl; red_tl_all) in "FULF_w". iDestruct "FULF_w" as "[%γκu DEAD_w]".
+              iModIntro. iRight. iFrame. iExists _. eauto.
             }
-            iModIntro. iLeft. iEval (red_tl; rewrite red_syn_inv). iFrame. iSplitR. auto.
-            iEval (unfold spinlockInv; red_tl_all; simpl). iRight. iFrame.
           }
-          { iEval (simpl; red_tl_all) in "FULF_w". iDestruct "FULF_w" as "(%γκu & DEAD_w)".
-            iEval (red_tl_all) in "DEAD_w". iPoseProof (OneShots.pending_not_shot with "LIVE_w DEAD_w") as "%F". inv F.
-          }
+          (* ELC continuation. *)
+          iModIntro. iEval (simpl; red_tl; simpl). iIntros "FC [A [%γκu B]]".
+          iEval (red_tl_all) in "B". iPoseProof "B" as "#DEAD_w". iClear "INV_SL".
+          iEval (red_tl_all; simpl; rewrite red_syn_inv) in "A". iDestruct "A" as "(#INV_SL & INV_SL_CLOSE & SL)".
+          iEval (unfold spinlockInv; red_tl_all; simpl) in "SL". iDestruct "SL" as "[(PTX & LX & EX) | (PTX & LX)]".
+          { iModIntro. iRight. iEval (red_tl_all; simpl; rewrite red_syn_inv). iSplitR. eauto. iFrame. }
+          iInv "INV_CL" as "CL" "INV_CL_CLOSE".
+          iEval (unfold clientSpinlock2_inv; simpl; red_tl_all; simpl) in "CL".
+          iDestruct "CL" as "[CL1 | [CL2 | [CL3 | CL4]]]".
+          + iExFalso. iDestruct "CL1" as "(LXw & _)". iPoseProof (AuthExcls.b_w_eq with "LX LXw") as "%F". inv F.
+          + iExFalso. iDestruct "CL2" as "(_ & _ & [% CL2])". iEval (red_tl) in "CL2". iDestruct "CL2" as "[% CL2]".
+            iEval (red_tl_all; simpl) in "CL2". iDestruct "CL2" as "(_ & LIVE_w & DEAD_l2 & _)".
+            iPoseProof (OneShots.shot_agree with "DEAD_l DEAD_l2") as "%EQ". subst x1.
+            iPoseProof (OneShots.pending_not_shot with "LIVE_w DEAD_w") as "%F". inv F.
+          + iDestruct "CL3" as "(LXw & PTD & % & CL3)". iEval (red_tl) in "CL3". iDestruct "CL3" as "[%κu CL3]".
+            iEval (red_tl) in "CL3". iDestruct "CL3" as "[% CL3]".
+            iEval (red_tl_all; simpl) in "CL3". iDestruct "CL3" as "(#PROM_u & LIVE_u & #LINK_u & #DEAD_l2 & #DEAD_w2 & PASS)".
+            iPoseProof (OneShots.shot_agree with "DEAD_l DEAD_l2") as "%EQ". subst x0.
+            iPoseProof (OneShots.shot_agree with "DEAD_w DEAD_w2") as "%EQ". subst x1.
+            iMod (tpromise_progress with "[FC]") as "[PC_u | #FULF_u]".
+            { iFrame. iApply "PROM_u". }
+            { iMod (link_amplify with "[PC_u]") as "PC_s".
+              { iFrame. iApply "LINK_u". }
+              iMod ("INV_CL_CLOSE" with "[LXw PTD LIVE_u PASS]") as "_".
+              { iEval (unfold clientSpinlock2_inv; simpl; red_tl_all; simpl). do 2 iRight. iLeft. iFrame.
+                iExists _. iEval (red_tl_all). iExists _. iEval (red_tl_all). iExists _.
+                iEval (red_tl_all; simpl). iFrame. iSplit. iApply "PROM_u". iSplit; eauto.
+              }
+              iModIntro. iLeft. iEval (red_tl; rewrite red_syn_inv). iFrame.
+              { iSplitL. iSplitR. auto. iEval (unfold spinlockInv; red_tl_all; simpl). iRight. iFrame.
+                iExists _. iEval (red_tl_all). eauto.
+              }
+            }
+            { iEval (simpl; red_tl_all) in "FULF_u".
+              iPoseProof (OneShots.pending_not_shot with "LIVE_u FULF_u") as "%F". inv F.
+            }
+          + iExFalso. iDestruct "CL4" as "(LXw & _)". iPoseProof (AuthExcls.b_w_eq with "LX LXw") as "%F". inv F.
+
         - iDestruct "CL3" as "(LXw & PTD & %γκw & CL3)". iEval (red_tl) in "CL3". iDestruct "CL3" as "[%κu CL3]".
           iEval (red_tl) in "CL3". iDestruct "CL3" as "[%γκu CL3]".
           iEval (red_tl_all; simpl) in "CL3". iDestruct "CL3" as "(#PROM_u & LIVE_u & #LINK_u & #DEAD_l & #DEAD_w & PASS)".
@@ -283,8 +306,8 @@ Section SIM.
               iExists _. iEval (red_tl_all). iExists _. iEval (red_tl_all). iExists _.
               iEval (red_tl_all; simpl). iFrame. iSplit. iApply "PROM_u". iSplit; eauto.
             }
-            iModIntro. iLeft. iEval (red_tl; rewrite red_syn_inv). iFrame. iSplitR. auto.
-            iEval (unfold spinlockInv; red_tl_all; simpl). iRight. iFrame.
+            iModIntro. iLeft. iEval (red_tl; rewrite red_syn_inv). iFrame.
+            iSplitR. auto. iEval (unfold spinlockInv; red_tl_all; simpl). iRight. iFrame.
           }
           { iEval (simpl; red_tl_all) in "FULF_u".
             iPoseProof (OneShots.pending_not_shot with "LIVE_u FULF_u") as "%F". inv F.
@@ -318,13 +341,13 @@ Section SIM.
           }
           iPoseProof (duty_tpromise with "DUTY") as "#PROM_w".
           { ss. eauto. }
-          iPoseProof (pc_split _ _ 1 1 with "PC_spin") as "[PC_spin PC_spin2]".
-          iMod (link_new _ _ _ 0 1 with "[PC_spin2]") as "[#LINK_w _]".
-          { subst ℓl ℓL. iSplitR. iApply "LO_w". iFrame. }
+          (* iPoseProof (pc_split _ _ 1 1 with "PC_spin") as "[PC_spin PC_spin2]". *)
+          (* iMod (link_new _ _ _ 0 1 with "[PC_spin2]") as "[#LINK_w _]". *)
+          (* { subst ℓl ℓL. iSplitR. iApply "LO_w". iFrame. } *)
           iMod ("INV_CL_CLOSE" with "[LXw PTD LIVE_w2 PC_spin DUTY2 LO_l]") as "_".
           { iEval (unfold clientSpinlock2_inv; simpl; red_tl_all; simpl). iRight. iLeft. iFrame.
             iExists κw. iEval (red_tl_all). iExists γκw. iEval (red_tl_all; simpl). iFrame.
-            iSplit. auto. iSplit. auto. iSplit. auto. auto.
+            iSplit. auto. iSplit. auto. iExists ℓl. iEval (red_tl). subst. iSplit; auto.
           }
           iModIntro. iFrame. iExists κw. iEval (red_tl). iExists γκw. iEval (red_tl_all; simpl). iFrame. auto.
         - iExFalso. iDestruct "CL2" as "(LXw & _)". iPoseProof (AuthExcls.b_w_eq with "LX LXw") as "%F". inv F.
@@ -337,15 +360,139 @@ Section SIM.
       { iModIntro. subst P0 R0. iEval (red_tl_all). iIntros "A". iModIntro. iFrame. }
       { iModIntro. subst P0 R0. iEval (red_tl_all). iIntros "A". iModIntro. iFrame. }
     }
-    
-          
+
+    (* POST. *)
+    iEval (red_tl_all). iIntros (_) "[Q EX]". rred2r. subst Q0.
+    iEval (red_tl_all) in "Q". iDestruct "Q" as "[%κw Q]". iEval (red_tl_all) in "Q". iDestruct "Q" as "[%γκw Q]".
+    iEval (red_tl_all; simpl) in "Q". iDestruct "Q" as "(#DEAD_l & LIVE_w & DUTY & PC)".
+    iMod (pc_drop _ 1 _ _ 100 with "PC") as "PC".
+    Unshelve. 1,3: lia.
+    iApply (wpsim_yieldR_gen2 with "[DUTY PC]").
+    3:{ iFrame. iApply pcs_cons_fold. iFrame. }
+    1,2: lia.
+    iIntros "DUTY _ PCS". iEval (simpl) in "PCS".
+    iModIntro. rred2r.
+    iInv "INV_CL" as "CL" "INV_CL_CLOSE".
+    iEval (unfold clientSpinlock2_inv; simpl; red_tl_all; simpl) in "CL".
+    iDestruct "CL" as "[CL1 | [CL2 | [CL3 | CL4]]]".
+    { iExFalso. iDestruct "CL1" as "(_ & _ & _ & LIVE_l & _)".
+      iPoseProof (OneShots.pending_not_shot with "LIVE_l DEAD_l") as "%F". inv F.
+    }
+    { iDestruct "CL2" as "(LXw & PTD & %κw0 & CL2)". iEval (red_tl) in "CL2". iDestruct "CL2" as "[%γκw0 CL2]".
+      iEval (red_tl_all; simpl) in "CL2". iDestruct "CL2" as "(#PROM_w & LIVE_w2 & #DEAD_l2 & DUTY2 & PC_spin & LO_w)".
+      iDestruct "LO_w" as "[% LO]". iEval (red_tl; simpl) in "LO". iPoseProof "LO" as "[#LO %LAY]".
+      iPoseProof (OneShots.shot_agree with "DEAD_l DEAD_l2") as "%EQ". subst γκw0.
+      iApply (SCMem_store_fun_spec with "[PTD] [-]").
+      3:{ iFrame. eauto. }
+      lia.
+      { pose md_N_ClientSpinlock2_state_tgt. set_solver. }
+      iIntros (rv) "PTD". rred2. iApply wpsim_tauR. rred2r.
+      iMod (alloc_obligation ℓl 2) as "(%κu & LOu & PCu)".
+      iMod (OneShots.alloc) as "[%γκu LIVEu]".
+      iPoseProof (OneShots.pending_split with "[LIVEu]") as "[LIVEu LIVEu2]".
+      { iEval (rewrite Qp.div_2). iFrame. }
+      iEval (replace 2 with (1+1) by lia) in "PCu". iPoseProof (pc_split with "PCu") as "[PCu PCu2]".
+      iMod (pc_drop _ 1 _ _ 1 with "PCu2") as "PCu2".
+      Unshelve. 1,3: lia.
+      iMod (duty_add with "[DUTY2 PCu2] []") as "DUTY2".
+      { subst ℓl. iFrame. }
+      { instantiate (1:= (▿ γκu 0)%S). iModIntro. iEval (simpl; red_tl_all). iIntros "#A". auto. }
+      iPoseProof (duty_tpromise with "DUTY2") as "#PROMu".
+      { simpl. eauto. }
+      iMod (OneShots.pending_shot with "[LIVE_w LIVE_w2]") as "#DEADw".
+      { iEval (rewrite <- (Qp.div_2 1)). iApply (OneShots.pending_merge with "LIVE_w LIVE_w2"). }
+      iMod (link_new _ _ _ 0 with "[LOu PC_spin]") as "[#LINKu _]".
+      { iSplitL "LOu". iFrame. subst. iFrame. }
+      iMod ("INV_CL_CLOSE" with "[LXw PTD LIVEu DUTY2 PCu LIVEu2 EX]") as "_".
+      { iEval (unfold clientSpinlock2_inv; simpl; red_tl_all; simpl). do 2 iRight. iLeft. iFrame.
+        iExists γκw. iEval (red_tl). iExists κu. iEval (red_tl). iExists γκu. iEval (red_tl_all; simpl).
+        iSplitR. auto. iSplitL "LIVEu". iFrame. iSplitR. auto. iSplitR. auto. iSplitR. auto. iLeft. iFrame.
+      }
+      iMod (duty_fulfill with "[DUTY]") as "DUTY".
+      { iFrame. iEval (simpl; red_tl). iExists _. iEval (red_tl_all). eauto. }
+      iApply (wpsim_sync with "[DUTY]").
+      2:{ iFrame. }
+      Unshelve. lia. 2: auto.
+      iIntros "DUTY FC". rred2r. iApply wpsim_tauR. rred2r. lred2r.
+      iApply wpsim_ret.
+      2:{ iModIntro. iFrame. iPureIntro. auto. }
+      reflexivity.
+    }
+    { iDestruct "CL3" as "(LXw & PTD & %γκw0 & CL3)". iEval (red_tl) in "CL3". iDestruct "CL3" as "[%κu CL3]".
+      iEval (red_tl) in "CL3". iDestruct "CL3" as "[%γκu CL3]".
+      iEval (red_tl_all; simpl) in "CL3". iDestruct "CL3" as "(#PROM_u & LIVE_u & #LINK_u & #DEAD_l2 & #DEAD_w & PASS)".
+      iPoseProof (OneShots.shot_agree with "DEAD_l DEAD_l2") as "%EQ". subst γκw0.
+      iPoseProof (OneShots.pending_not_shot with "LIVE_w DEAD_w") as "%F". inv F.
+    }
+    { iDestruct "CL4" as "(LXw & PTD & %γκw0 & CL4)". iEval (red_tl) in "CL4". iDestruct "CL4" as "[%γκu CL4]".
+      iEval (red_tl_all; simpl) in "CL4". iDestruct "CL4" as "(#DEAD_l2 & #DEAD_w & _)".
+      iPoseProof (OneShots.shot_agree with "DEAD_l DEAD_l2") as "%EQ". subst γκw0.
+      iPoseProof (OneShots.pending_not_shot with "LIVE_w DEAD_w") as "%F". inv F.
+    }
+  Qed.
+
+  Lemma ClientSpinlock2_thread2_sim
+        tid2 n
+        ℓL ℓl
+        (LAYER_L : ℓL = 3)
+        (LAYER_l : ℓl = 2)
+    :
+    ⊢ ⟦(∀ (γX γe κs κl γκl γr : τ{nat, 1+n}),
+           ((⤉ syn_inv n N_ClientSpinlock2 (clientSpinlock2_inv n tid2 ℓL ℓl γX γe κs κl γκl γr))
+              ∗ (syn_tgt_interp_as n sndl (fun m => (s_memory_black m)))
+              ∗ (⤉ isSpinlock n X γX γe κs ℓL)
+              ∗ (⤉ -[κl](0)-◇ (∃ (γκw : τ{nat}), ▿ γκl γκw))
+              ∗ (∃ (ℓl : τ{nat}), ◆[κl, ℓl])
+              ∗ TID(tid2)
+              ∗ (⤉ △ γr 1))
+             -∗
+             syn_wpsim (S n) tid2 ⊤
+             (fun rs rt => (⤉(syn_term_cond n tid2 _ rs rt))%S)
+             false false
+             (fn2th ClientSpinlock2Spec.module "thread2" (tt ↑))
+             (fn2th ClientSpinlock2.module "thread2" (tt ↑)))%S, 1+n⟧.
+  Proof.
+    iIntros.
+    red_tl. iIntros (γX). red_tl. iIntros (γe). red_tl. iIntros (κs).
+    red_tl. iIntros (κl). red_tl. iIntros (γκl). red_tl. iIntros (γr).
+    iEval (red_tl_all; simpl; rewrite red_syn_inv; rewrite red_syn_wpsim; rewrite red_syn_tgt_interp_as).
+    iIntros "(#INV_CL & #MEM & #ISL & #PROMl & [%ℓl0 LOl] & TID & LIVE_r)".
+    iEval (red_tl; simpl) in "LOl". iPoseProof "LOl" as "#LOl".
+    unfold fn2th. simpl. unfold thread2, ClientSpinlock2Spec.thread2. rred2r. lred2r.
 
 
-        
-          
 
 
 
+  Definition clientSpinlock2_inv n (tid2 : thread_id) (ℓL ℓl : nat) (γX γe κs : nat) (κl γκl : nat) (γr : nat) : sProp n :=
+    (
+      ((○ γX 0) ∗ (D ↦ 0)
+                ∗ (-[κl](0)-◇ (∃ (γκw : τ{nat}), ▿ γκl γκw)) ∗ (△ γκl (1/2))
+                ∗ (Duty(tid2) [])
+                ∗ ◇[κs](ℓL, 1)
+                ∗ (∃ (ℓl : τ{nat}), ◆[κl, ℓl])
+      )
+      ∨
+        ((○ γX 1) ∗ (D ↦ 0)
+                  ∗ (∃ (κw γκw : τ{nat}),
+                        (-[κw](0)-◇ (∃ (γκu : τ{nat}), (▿ γκw γκu)))
+                          ∗ (△ γκw (1/2)) ∗ (▿ γκl γκw)
+                          ∗ (Duty(tid2) [])
+                          ∗ ◇[κs](ℓL, 1)
+                          ∗ (∃ (ℓw : τ{nat}), ◆[κw, ℓw] ∗ ⌜ℓw <= ℓL⌝))
+        )
+      ∨
+        ((○ γX 1) ∗ (D ↦ 1)
+                  ∗ (∃ (γκw κu γκu : τ{nat}),
+                        (-[κu](0)-◇ (▿ γκu 0))
+                          ∗ (△ γκu (1/2)) ∗ (κu -(0)-◇ κs) ∗ (▿ γκl γκw) ∗ (▿ γκw γκu)
+                          ∗ ((Duty(tid2) [(κu, 0, (▿ γκu 0))] ∗ ◇[κu](ℓl, 1) ∗ (△ γκu (1/2)) ∗ (EX γe tt)) ∨ (▿ γr 0)))
+        )
+      ∨
+        ((○ γX 0) ∗ (D ↦ 1)
+                  ∗ (∃ (γκw γκu : τ{nat}),
+                        (▿ γκl γκw) ∗ (▿ γκw γκu) ∗ (▿ γr 0) ∗ (▿ γκu 0)))
+    )%S.
 
 End SIM.
 
